Imp ver.1.1: no more while/ ge fixed/ new stmt: cmp

theories/Imp.v
@@ -61,19 +61,19 @@ Inductive stmt : Type :=
 | Assign (x : var) (e : expr)    (* x = e *)
 | Seq    (a b : stmt)            (* a ; b *)
 | If     (i : expr) (t e : stmt) (* if (i) then { t } else { e } *)
-| While  (t : expr) (b : stmt)   (* while (t) { b } *)
 | Skip                           (* ; *)
 | CallFun1 (x : var) (f : gname) (args : list expr) (* x = f(args), call by name *)
-| CallFun2 (f : gname) (args : list expr) (* f(args) *)
-| CallPtr1 (x : var) (p : expr) (args : list expr)  (* x = f(args), call by pointer *)
-| CallPtr2 (p : expr) (args : list expr) (* f(args) *)
+| CallFun2 (f : gname) (args : list expr)           (* f(args) *)
+| CallPtr1 (x : var) (p : expr) (args : list expr)  (* x = f(args), by pointer*)
+| CallPtr2 (p : expr) (args : list expr)            (* f(args) *)
 | CallSys1 (x : var) (f : gname) (args : list expr) (* x = f(args), system call *)
-| CallSys2 (f : gname) (args : list expr) (* f(args) *)
-| Return1 (e : expr)              (* return e *)
-| Return2                         (* return *)
-| AddrOf (x : var) (X : gname)   (* x = &X *)
-| Load (x : var) (p : expr)      (* x = *p *)
-| Store (p : expr) (v : expr)    (* *p = v *)
+| CallSys2 (f : gname) (args : list expr)           (* f(args) *)
+| Return1 (e : expr)                                (* return e *)
+| Return2                                           (* return *)
+| AddrOf (x : var) (X : gname)         (* x = &X *)
+| Load (x : var) (p : expr)            (* x = *p *)
+| Store (p : expr) (v : expr)          (* *p = v *)
+| Cmp (x : var) (a : expr) (b : expr)  (* memory accessing equality comparison *)
 .
 
 (** information of a function *)
@@ -138,27 +138,20 @@ Section Denote.
       v <- denote_expr e;; trigger (SetVar x v);; Ret Vundef
     | Seq a b =>
       denote_stmt a;; denote_stmt b
-
     | If i t e =>
       v <- denote_expr i;; `b: bool <- (is_true v)?;;
       if b then (denote_stmt t) else (denote_stmt e)
-
-    | While t b =>
-      while (v <- denote_expr t;; `c: bool <- (is_true v)?;;
-      if c then (denote_stmt b;; Ret (inl tt)) else (Ret (inr Vundef)))
-
     | Skip => Ret Vundef
 
     | CallFun1 x f args =>
-      if (String.string_dec f "load" || String.string_dec f "store")
+      if (String.string_dec f "load" || String.string_dec f "store" || String.string_dec f "cmp")
       then triggerUB
       else
         eval_args <- denote_exprs args [];;
         v <- trigger (Call f (eval_args↑));; v <- unwrapN (v↓);;
         trigger (SetVar x v);; Ret Vundef
-
     | CallFun2 f args =>
-      if (String.string_dec f "load" || String.string_dec f "store")
+      if (String.string_dec f "load" || String.string_dec f "store" || String.string_dec f "cmp")
       then triggerUB
       else
         eval_args <- denote_exprs args [];;
@@ -166,16 +159,15 @@ Section Denote.
 
     | CallPtr1 x e args =>
       p <- denote_expr e;; f <- trigger (GetName p);;
-      if (String.string_dec f "load" || String.string_dec f "store")
+      if (String.string_dec f "load" || String.string_dec f "store" || String.string_dec f "cmp")
       then triggerUB
       else
         eval_args <- denote_exprs args [];;
         v <- trigger (Call f (eval_args↑));; v <- unwrapN (v↓);;
         trigger (SetVar x v);; Ret Vundef
-
     | CallPtr2 e args =>
       p <- denote_expr e;; f <- trigger (GetName p);;
-      if (String.string_dec f "load" || String.string_dec f "store")
+      if (String.string_dec f "load" || String.string_dec f "store" || String.string_dec f "cmp")
       then triggerUB
       else
         eval_args <- denote_exprs args [];;
@@ -185,7 +177,6 @@ Section Denote.
       eval_args <- denote_exprs args [];;
       v <- trigger (Syscall f eval_args top1);;
       trigger (SetVar x v);; Ret Vundef
-
     | CallSys2 f args =>
       eval_args <- denote_exprs args [];;
       trigger (Syscall f eval_args top1);; Ret Vundef
@@ -202,6 +193,10 @@ Section Denote.
     | Store pe ve =>
       p <- denote_expr pe;; v <- denote_expr ve;;
       trigger (Call "store" ([p ; v]↑));; Ret Vundef
+    | Cmp x ae be =>
+      a <- denote_expr ae;; b <- denote_expr be;;
+      v <- trigger (Call "cmp" ([a ; b]↑));; v <- unwrapN (v↓);;
+      trigger (SetVar x v);; Ret Vundef
 
     end.
 
@@ -215,20 +210,20 @@ Section Interp.
   Context `{Σ: GRA.t}.
   Definition effs := GlobEnv +' ImpState +' Es.
 
-  Definition handle_GlobEnv {eff} `{eventE -< eff} : GlobEnv ~> stateT SkEnv.t (itree eff) :=
-    fun _ e ge =>
+  Definition handle_GlobEnv {eff} `{eventE -< eff} (ge: SkEnv.t) : GlobEnv ~> (itree eff) :=
+    fun _ e =>
       match e with
       | GetPtr X =>
-        r <- (ge.(SkEnv.id2blk) X)?;; Ret (ge, Vptr r 0)
+        r <- (ge.(SkEnv.id2blk) X)?;; Ret (Vptr r 0)
       | GetName p =>
         match p with
-        | Vptr n z => x <- (ge.(SkEnv.blk2id) n)?;; Ret (ge, x)
+        | Vptr n 0 => x <- (ge.(SkEnv.blk2id) n)?;; Ret (x)
         | _ => triggerUB
         end
       end.
 
-  Definition interp_GlobEnv {eff} `{eventE -< eff}: itree (GlobEnv +' eff) ~> stateT SkEnv.t (itree eff) :=
-    State.interp_state (case_ handle_GlobEnv ModSem.pure_state).
+  Definition interp_GlobEnv {eff} `{eventE -< eff} (ge: SkEnv.t) : itree (GlobEnv +' eff) ~> (itree eff) :=
+    interp (case_ (handle_GlobEnv ge) ((fun T e => trigger e) : eff ~> itree eff)).
 
   (** function local environment *)
   Definition lenv := alist var val.
@@ -243,7 +238,7 @@ Section Interp.
     State.interp_state (case_ handle_ImpState ModSem.pure_state).
 
   Definition interp_imp ge le (itr : itree effs val) :=
-    interp_ImpState (interp_GlobEnv itr ge) le.
+    interp_ImpState (interp_GlobEnv ge itr) le.
   
   Fixpoint init_lenv xs : lenv :=
     match xs with
@@ -264,7 +259,7 @@ Section Interp.
   Definition eval_imp (ge: SkEnv.t) (f: function) (args: list val) : itree Es val :=
     match (init_args f.(fn_params) args []) with
     | Some iargs =>
-      '(_, (_, retv)) <- (interp_imp ge (iargs++(init_lenv f.(fn_vars))) (denote_stmt f.(fn_body)));; Ret retv
+      '(_, retv) <- (interp_imp ge (iargs++(init_lenv f.(fn_vars))) (denote_stmt f.(fn_body)));; Ret retv
     | None => triggerUB
     end
   .
@@ -357,13 +352,6 @@ Module ImpNotations.
        format
          "'[v ' 'if#'  i '/' '[' 'then#'  t  ']' '/' '[' 'else#'  e ']' '/' 'fi#' ']'").
 
-  Notation "'while#' t 'do#' b 'end#'" :=
-    (While t b)
-      (at level 100,
-       right associativity,
-       format
-         "'[v  ' 'while#'  t  'do#' '/' '[v' b  ']' ']' '/' 'end#'").
-
   Notation "'skip#'" :=
     (Skip) (at level 100): stmt_scope.
 
@@ -408,16 +396,15 @@ Module ImpNotations.
   Notation "'*' p '=#' v" :=
     (Store p v) (at level 60): stmt_scope.
 
+  Notation "x '=#' '(' a '==' b ')'" :=
+    (Cmp x a b) (at level 60): stmt_scope.
+
   Notation "x '=#' 'alloc#' s" :=
     (CallFun1 x "alloc" [s])
       (at level 60): stmt_scope.
 
   Notation "'free#' p" :=
     (CallFun2 "free" [p])
-      (at level 60): stmt_scope.
-
-  Notation "x '=#' '(' a '==' b ')'" :=
-    (CallFun1 x "cmp" [a ; b])
       (at level 60): stmt_scope.
 
 End ImpNotations.
@@ -434,10 +421,11 @@ Section Example_Extract.
   Local Open Scope stmt_scope.
 
   Definition factorial : stmt :=
-    "output" =# 1%Z ;#
-    while# "input"
-    do# "output" =# "output" * "input";#
-       "input"  =# "input" - 1%Z end#;#
+    if# "input"
+    then# "output" =@ "factorial" ["input" - 1%Z] ;#
+          "output" =# "input" * "output"
+    else# "output" =# 1%Z
+    fi#;#
     ret# "output".
 
   Definition factorial_fundef : function := {|
@@ -475,122 +463,123 @@ Section PROOFS.
 
   (* expr *)
   Lemma denote_expr_Var
-        ge0 le0 v
+        ge le0 v
     :
-      interp_imp ge0 le0 (denote_expr (Var v)) =
-      interp_imp ge0 le0 (trigger (GetVar v)).
+      interp_imp ge le0 (denote_expr (Var v)) =
+      interp_imp ge le0 (trigger (GetVar v)).
   Proof. reflexivity. Qed.
 
   Lemma denote_expr_Lit
-        ge0 le0 n
+        ge le0 n
     :
-      interp_imp ge0 le0 (denote_expr (Lit n)) =
-      interp_imp ge0 le0 (Ret n).
+      interp_imp ge le0 (denote_expr (Lit n)) =
+      interp_imp ge le0 (Ret n).
   Proof. reflexivity. Qed.
 
   Lemma denote_expr_Plus
-        ge0 le0 a b
+        ge le0 a b
     :
-      interp_imp ge0 le0 (denote_expr (Plus a b)) =
-      interp_imp ge0 le0 (l <- denote_expr a ;; r <- denote_expr b ;; (vadd l r)?).
+      interp_imp ge le0 (denote_expr (Plus a b)) =
+      interp_imp ge le0 (l <- denote_expr a ;; r <- denote_expr b ;; (vadd l r)?).
   Proof. reflexivity. Qed.
 
   Lemma denote_expr_Minus
-        ge0 le0 a b
+        ge le0 a b
     :
-      interp_imp ge0 le0 (denote_expr (Minus a b)) =
-      interp_imp ge0 le0 (l <- denote_expr a ;; r <- denote_expr b ;; (vsub l r)?).
+      interp_imp ge le0 (denote_expr (Minus a b)) =
+      interp_imp ge le0 (l <- denote_expr a ;; r <- denote_expr b ;; (vsub l r)?).
   Proof. reflexivity. Qed.
 
   Lemma denote_expr_Mult
-        ge0 le0 a b
+        ge le0 a b
     :
-      interp_imp ge0 le0 (denote_expr (Mult a b)) =
-      interp_imp ge0 le0 (l <- denote_expr a ;; r <- denote_expr b ;; (vmul l r)?).
+      interp_imp ge le0 (denote_expr (Mult a b)) =
+      interp_imp ge le0 (l <- denote_expr a ;; r <- denote_expr b ;; (vmul l r)?).
   Proof. reflexivity. Qed.
 
   (* stmt *)
   Lemma denote_stmt_Assign
-        ge0 le0 x e
+        ge le0 x e
     :
-      interp_imp ge0 le0 (denote_stmt (Assign x e)) =
-      interp_imp ge0 le0 (v <- denote_expr e ;; trigger (SetVar x v) ;; Ret Vundef).
+      interp_imp ge le0 (denote_stmt (Assign x e)) =
+      interp_imp ge le0 (v <- denote_expr e ;; trigger (SetVar x v) ;; Ret Vundef).
   Proof. reflexivity. Qed.
   
   Lemma denote_stmt_Seq
-        ge0 le0 a b
+        ge le0 a b
     :
-      interp_imp ge0 le0 (denote_stmt (Seq a b)) =
-      interp_imp ge0 le0 (denote_stmt a ;; denote_stmt b).
+      interp_imp ge le0 (denote_stmt (Seq a b)) =
+      interp_imp ge le0 (denote_stmt a ;; denote_stmt b).
   Proof. reflexivity. Qed.
 
   Lemma denote_stmt_If
-        ge0 le0 i t e
+        ge le0 i t e
     :
-      interp_imp ge0 le0 (denote_stmt (If i t e)) =
-      interp_imp ge0 le0 (v <- denote_expr i ;; `b: bool <- (is_true v)? ;;
+      interp_imp ge le0 (denote_stmt (If i t e)) =
+      interp_imp ge le0 (v <- denote_expr i ;; `b: bool <- (is_true v)? ;;
       if b then (denote_stmt t) else (denote_stmt e)).
   Proof. reflexivity. Qed.
 
-  Lemma denote_stmt_While
-        ge0 le0 t b
-    :
-      interp_imp ge0 le0 (denote_stmt (While t b)) =
-      interp_imp ge0 le0 (while (v <- denote_expr t ;; `c: bool <- (is_true v)? ;;
-      if c then (denote_stmt b ;; Ret (inl tt)) else (Ret (inr Vundef)))).
-  Proof. reflexivity. Qed.
-
   Lemma denote_stmt_Skip
-        ge0 le0
+        ge le0
     :
-      interp_imp ge0 le0 (denote_stmt (Skip)) =
-      interp_imp ge0 le0 (Ret Vundef).
+      interp_imp ge le0 (denote_stmt (Skip)) =
+      interp_imp ge le0 (Ret Vundef).
   Proof. reflexivity. Qed.
 
   Lemma denote_stmt_Return1
-        ge0 le0 e
+        ge le0 e
     :
-      interp_imp ge0 le0 (denote_stmt (Return1 e)) =
-      interp_imp ge0 le0 (v <- denote_expr e;; Ret v).
+      interp_imp ge le0 (denote_stmt (Return1 e)) =
+      interp_imp ge le0 (v <- denote_expr e;; Ret v).
   Proof. reflexivity. Qed.
 
   Lemma denote_stmt_Return2
-        ge0 le0
+        ge le0
     :
-      interp_imp ge0 le0 (denote_stmt (Return2)) =
-      interp_imp ge0 le0 (Ret Vundef).
+      interp_imp ge le0 (denote_stmt (Return2)) =
+      interp_imp ge le0 (Ret Vundef).
   Proof. reflexivity. Qed.
 
   Lemma denote_stmt_AddrOf
-        ge0 le0 x X
+        ge le0 x X
     :
-      interp_imp ge0 le0 (denote_stmt (AddrOf x X)) =
-      interp_imp ge0 le0 (v <- trigger (GetPtr X);; trigger (SetVar x v);; Ret Vundef).
+      interp_imp ge le0 (denote_stmt (AddrOf x X)) =
+      interp_imp ge le0 (v <- trigger (GetPtr X);; trigger (SetVar x v);; Ret Vundef).
   Proof. reflexivity. Qed.
 
   Lemma denote_stmt_Load
-        ge0 le0 x pe
+        ge le0 x pe
     :
-      interp_imp ge0 le0 (denote_stmt (Load x pe)) =
-      interp_imp ge0 le0 (p <- denote_expr pe;;
+      interp_imp ge le0 (denote_stmt (Load x pe)) =
+      interp_imp ge le0 (p <- denote_expr pe;;
       v <- trigger (Call "load" (p↑));; v <- unwrapN(v↓);;
       trigger (SetVar x v);; Ret Vundef).
   Proof. reflexivity. Qed.
 
   Lemma denote_stmt_Store
-        ge0 le0 pe ve
+        ge le0 pe ve
     :
-      interp_imp ge0 le0 (denote_stmt (Store pe ve)) =
-      interp_imp ge0 le0 (p <- denote_expr pe;; v <- denote_expr ve;;
+      interp_imp ge le0 (denote_stmt (Store pe ve)) =
+      interp_imp ge le0 (p <- denote_expr pe;; v <- denote_expr ve;;
       trigger (Call "store" ([p ; v]↑));; Ret Vundef).
   Proof. reflexivity. Qed.
 
-  Lemma denote_stmt_CallFun1
-        ge0 le0 x f args
+  Lemma denote_stmt_Cmp
+        ge le0 x ae be
     :
-      interp_imp ge0 le0 (denote_stmt (CallFun1 x f args)) =
-      interp_imp ge0 le0 (
-      if (String.string_dec f "load" || String.string_dec f "store")
+      interp_imp ge le0 (denote_stmt (Cmp x ae be)) =
+      interp_imp ge le0 ( a <- denote_expr ae;; b <- denote_expr be;;
+      v <- trigger (Call "cmp" ([a ; b]↑));; v <- unwrapN (v↓);;
+      trigger (SetVar x v);; Ret Vundef).
+  Proof. reflexivity. Qed.
+
+  Lemma denote_stmt_CallFun1
+        ge le0 x f args
+    :
+      interp_imp ge le0 (denote_stmt (CallFun1 x f args)) =
+      interp_imp ge le0 (
+      if (String.string_dec f "load" || String.string_dec f "store" || String.string_dec f "cmp")
       then triggerUB
       else
         eval_args <- (denote_exprs args []);;
@@ -599,11 +588,11 @@ Section PROOFS.
   Proof. reflexivity. Qed.
 
   Lemma denote_stmt_CallFun2
-        ge0 le0 f args
+        ge le0 f args
     :
-      interp_imp ge0 le0 (denote_stmt (CallFun2 f args)) =
-      interp_imp ge0 le0 (
-      if (String.string_dec f "load" || String.string_dec f "store")
+      interp_imp ge le0 (denote_stmt (CallFun2 f args)) =
+      interp_imp ge le0 (
+      if (String.string_dec f "load" || String.string_dec f "store" || String.string_dec f "cmp")
       then triggerUB
       else
         eval_args <- (denote_exprs args []);;
@@ -611,12 +600,12 @@ Section PROOFS.
   Proof. reflexivity. Qed.
 
   Lemma denote_stmt_CallPtr1
-        ge0 le0 x e args
+        ge le0 x e args
     :
-      interp_imp ge0 le0 (denote_stmt (CallPtr1 x e args)) =
-      interp_imp ge0 le0 (
+      interp_imp ge le0 (denote_stmt (CallPtr1 x e args)) =
+      interp_imp ge le0 (
       p <- denote_expr e;; f <- trigger (GetName p);;
-      if (String.string_dec f "load" || String.string_dec f "store")
+      if (String.string_dec f "load" || String.string_dec f "store" || String.string_dec f "cmp")
       then triggerUB
       else
         eval_args <- (denote_exprs args []);;
@@ -625,12 +614,12 @@ Section PROOFS.
   Proof. reflexivity. Qed.
   
   Lemma denote_stmt_CallPtr2
-        ge0 le0 e args
+        ge le0 e args
     :
-      interp_imp ge0 le0 (denote_stmt (CallPtr2 e args)) =
-      interp_imp ge0 le0 (
+      interp_imp ge le0 (denote_stmt (CallPtr2 e args)) =
+      interp_imp ge le0 (
       p <- denote_expr e;; f <- trigger (GetName p);;
-      if (String.string_dec f "load" || String.string_dec f "store")
+      if (String.string_dec f "load" || String.string_dec f "store") || String.string_dec f "cmp"
       then triggerUB
       else
         eval_args <- (denote_exprs args []);;
@@ -638,20 +627,20 @@ Section PROOFS.
   Proof. reflexivity. Qed.
 
   Lemma denote_stmt_CallSys1
-        ge0 le0 x f args
+        ge le0 x f args
     :
-      interp_imp ge0 le0 (denote_stmt (CallSys1 x f args)) =
-      interp_imp ge0 le0 (
+      interp_imp ge le0 (denote_stmt (CallSys1 x f args)) =
+      interp_imp ge le0 (
       eval_args <- (denote_exprs args []);;
       v <- trigger (Syscall f eval_args top1);;
       trigger (SetVar x v);; Ret Vundef).
   Proof. reflexivity. Qed.
 
   Lemma denote_stmt_CallSys2
-        ge0 le0 f args
+        ge le0 f args
     :
-      interp_imp ge0 le0 (denote_stmt (CallSys2 f args)) =
-      interp_imp ge0 le0 (
+      interp_imp ge le0 (denote_stmt (CallSys2 f args)) =
+      interp_imp ge le0 (
       eval_args <- (denote_exprs args []);;
       trigger (Syscall f eval_args top1);; Ret Vundef).
   Proof. reflexivity. Qed.
@@ -659,58 +648,58 @@ Section PROOFS.
   (* interp_imp *)
 
   Lemma interp_imp_bind
-        itr ktr ge0 le0
+        itr ktr ge le0
     :
-      interp_imp ge0 le0 (v <- itr ;; ktr v) =
-      '(le1, (ge1, v)) <- interp_imp ge0 le0 itr ;;
-      interp_imp ge1 le1 (ktr v).
+      interp_imp ge le0 (v <- itr ;; ktr v) =
+      '(le1, v) <- interp_imp ge le0 itr ;;
+      interp_imp ge le1 (ktr v).
   Proof.
     unfold interp_imp. unfold interp_GlobEnv.
     unfold interp_ImpState. grind. des_ifs.
   Qed.
 
   Lemma interp_imp_tau
-        itr ge0 le0
+        itr ge le0
     :
-      interp_imp ge0 le0 (tau;; itr) =
-      tau;; interp_imp ge0 le0 itr.
+      interp_imp ge le0 (tau;; itr) =
+      tau;; interp_imp ge le0 itr.
   Proof.
     unfold interp_imp, interp_ImpState, interp_GlobEnv.
     grind.
   Qed.
 
   Lemma interp_imp_Ret
-        ge0 le0 v
+        ge le0 v
     :
-      interp_imp ge0 le0 (Ret v) = Ret (le0, (ge0, v)).
+      interp_imp ge le0 (Ret v) = Ret (le0, v).
   Proof.
     unfold interp_imp, interp_ImpState, interp_GlobEnv.
     grind.
   Qed.
 
   Lemma interp_imp_triggerUB
-        ge0 le0
+        ge le0
     :
-      (interp_imp ge0 le0 (triggerUB) : itree Es _) = triggerUB.
+      (interp_imp ge le0 (triggerUB) : itree Es _) = triggerUB.
   Proof.
     unfold interp_imp, interp_ImpState, interp_GlobEnv, pure_state, triggerUB.
-    grind.
+    grind. rewrite interp_trigger. grind.
   Qed.
 
   Lemma interp_imp_triggerNB
-        ge0 le0
+        ge le0
     :
-      (interp_imp ge0 le0 (triggerNB) : itree Es _) = triggerNB.
+      (interp_imp ge le0 (triggerNB) : itree Es _) = triggerNB.
   Proof.
     unfold interp_imp, interp_ImpState, interp_GlobEnv, pure_state, triggerNB.
-    grind.
+    grind. rewrite interp_trigger. grind.
   Qed.
 
   Lemma interp_imp_unwrapU
-        x ge0 le0
+        x ge le0
     :
-      interp_imp ge0 le0 (unwrapU x) =
-      x <- unwrapU x;; Ret (le0, (ge0, x)).
+      interp_imp ge le0 (unwrapU x) =
+      x <- unwrapU x;; Ret (le0, x).
   Proof.
     unfold unwrapU. des_ifs.
     - rewrite interp_imp_Ret. ired. ss.
@@ -719,10 +708,10 @@ Section PROOFS.
   Qed.
 
   Lemma interp_imp_unwrapN
-        x ge0 le0
+        x ge le0
     :
-      interp_imp ge0 le0 (unwrapN x) =
-      x <- unwrapN x;; Ret (le0, (ge0, x)).
+      interp_imp ge le0 (unwrapN x) =
+      x <- unwrapN x;; Ret (le0, x).
   Proof.
     unfold unwrapN. des_ifs.
     - rewrite interp_imp_Ret. ired. ss.
@@ -731,115 +720,117 @@ Section PROOFS.
   Qed.
 
   Lemma interp_imp_GetPtr
-        ge0 le0 X
+        ge le0 X
     :
-      interp_imp ge0 le0 (trigger (GetPtr X)) =
-      r <- (ge0.(SkEnv.id2blk) X)? ;; tau;; Ret (le0, (ge0, Vptr r 0)).
+      interp_imp ge le0 (trigger (GetPtr X)) =
+      r <- (ge.(SkEnv.id2blk) X)? ;; tau;; Ret (le0, Vptr r 0).
   Proof.
     unfold interp_imp, interp_GlobEnv, interp_ImpState, unwrapU.
     des_ifs; grind.
-    - unfold unwrapU. des_ifs. grind.
-    - unfold unwrapU. des_ifs. unfold triggerUB, pure_state. grind.
+    - rewrite interp_trigger. grind.
+      unfold unwrapU. des_ifs. grind.
+    - rewrite interp_trigger. grind.
+      unfold unwrapU. des_ifs. unfold triggerUB, pure_state. grind.
   Qed.
 
   Lemma interp_imp_GetVar
-        ge0 le0 x
+        ge le0 x
     :
-      (interp_imp ge0 le0 (trigger (GetVar x)) : itree Es _) =
-      r <- unwrapU (alist_find _ x le0);; tau;; tau;; Ret (le0, (ge0, r)).
+      (interp_imp ge le0 (trigger (GetVar x)) : itree Es _) =
+      r <- unwrapU (alist_find _ x le0);; tau;; tau;; Ret (le0, r).
   Proof.
     unfold interp_imp, interp_ImpState, interp_GlobEnv.
-    grind. unfold unwrapU, pure_state, triggerUB. des_ifs; grind.
-    - unfold unwrapU; grind.
-    - unfold unwrapU, triggerUB. grind.
+    rewrite interp_trigger. grind.
   Qed.
 
   Lemma interp_imp_SetVar_Vundef
-        ge0 le0 x v
+        ge le0 x v
     :
-      interp_imp ge0 le0 (trigger (SetVar x v) ;; Ret Vundef) =
-      tau;; tau;; Ret (alist_add _ x v le0, (ge0, Vundef)).
+      interp_imp ge le0 (trigger (SetVar x v) ;; Ret Vundef) =
+      tau;; tau;; Ret (alist_add _ x v le0, Vundef).
   Proof.
     unfold interp_imp, interp_GlobEnv, interp_ImpState. grind.
-    unfold pure_state. grind.
+    rewrite interp_trigger. grind.
   Qed.
 
   Lemma interp_imp_Call_only
-        ge0 le0 f args
+        ge le0 f args
     :
-      interp_imp ge0 le0 (trigger (Call f args);; Ret Vundef) =
-      trigger (Call f args);; tau;; tau;; Ret (le0, (ge0, Vundef)).
+      interp_imp ge le0 (trigger (Call f args);; Ret Vundef) =
+      trigger (Call f args);; tau;; tau;; Ret (le0, Vundef).
   Proof.
     unfold interp_imp, interp_GlobEnv, interp_ImpState. grind.
-    unfold pure_state. grind.
+    unfold pure_state. rewrite interp_trigger. grind.
   Qed.
 
   Lemma interp_imp_Call_ret
-        ge0 le0 f args x
+        ge le0 f args x
     :
-      interp_imp ge0 le0
+      interp_imp ge le0
                  (v <- trigger (Call f args);; v <- unwrapN (v↓);;
                   trigger (SetVar x v);; Ret Vundef) =
       v <- trigger (Call f args);;
       tau;; tau;; v <- unwrapN (v↓);;
-      tau;; tau;; Ret (alist_add _ x v le0, (ge0, Vundef)).
+      tau;; tau;; Ret (alist_add _ x v le0, Vundef).
   Proof.
     unfold interp_imp, interp_GlobEnv, interp_ImpState. grind.
-    unfold pure_state. grind.
+    unfold pure_state. rewrite interp_trigger. grind.
     unfold unwrapN. des_ifs; grind.
-    unfold triggerNB; grind.
+    - rewrite interp_trigger. grind.
+    - unfold triggerNB. grind. rewrite interp_trigger. grind.
   Qed.
 
   Lemma interp_imp_Syscall_only
-        ge0 le0 f args
+        ge le0 f args
     :
-      interp_imp ge0 le0 (trigger (Syscall f args top1);; Ret Vundef) =
-      trigger (Syscall f args top1);; tau;; tau;; Ret (le0, (ge0, Vundef)).
+      interp_imp ge le0 (trigger (Syscall f args top1);; Ret Vundef) =
+      trigger (Syscall f args top1);; tau;; tau;; Ret (le0, Vundef).
   Proof.
     unfold interp_imp, interp_GlobEnv, interp_ImpState. grind.
-    unfold pure_state. grind.
+    unfold pure_state. rewrite interp_trigger. grind.
   Qed.
 
   Lemma interp_imp_Syscall_ret
-        ge0 le0 f args x
+        ge le0 f args x
     :
-      interp_imp ge0 le0
+      interp_imp ge le0
                  (v <- trigger (Syscall f args top1);;
                   trigger (SetVar x v);; Ret Vundef) =
       v <- trigger (Syscall f args top1);;
       tau;; tau;; tau;; tau;;
-      Ret (alist_add _ x v le0, (ge0, Vundef)).
+      Ret (alist_add _ x v le0, Vundef).
   Proof.
     unfold interp_imp, interp_GlobEnv, interp_ImpState. grind.
-    unfold pure_state. grind.
+    unfold pure_state. rewrite interp_trigger. grind.
+    rewrite interp_trigger. grind.
   Qed.
 
   Lemma interp_imp_expr_Var
-        ge0 le0 v
+        ge le0 v
     :
-      interp_imp ge0 le0 (denote_expr (Var v)) =
-      r <- unwrapU (alist_find _ v le0);; tau;; tau;; Ret (le0, (ge0, r)).
+      interp_imp ge le0 (denote_expr (Var v)) =
+      r <- unwrapU (alist_find _ v le0);; tau;; tau;; Ret (le0, r).
   Proof.
     apply interp_imp_GetVar.
   Qed.
 
   Lemma interp_imp_expr_Lit
-        ge0 le0 n
+        ge le0 n
     :
-      interp_imp ge0 le0 (denote_expr (Lit n)) =
-      Ret (le0, (ge0, n)).
+      interp_imp ge le0 (denote_expr (Lit n)) =
+      Ret (le0, n).
   Proof.
     rewrite denote_expr_Lit. apply interp_imp_Ret.
   Qed.
 
   Lemma interp_imp_expr_Plus
-        ge0 le0 a b
+        ge le0 a b
     :
-      interp_imp ge0 le0 (denote_expr (Plus a b)) =
-      '(le1, (ge1, l)) <- interp_imp ge0 le0 (denote_expr a) ;;
-      '(le2, (ge2, r)) <- interp_imp ge1 le1 (denote_expr b) ;;
+      interp_imp ge le0 (denote_expr (Plus a b)) =
+      '(le1, l) <- interp_imp ge le0 (denote_expr a) ;;
+      '(le2, r) <- interp_imp ge le1 (denote_expr b) ;;
       v <- (vadd l r)? ;;
-      Ret (le2, (ge2, v))
+      Ret (le2, v)
   .
   Proof.
     rewrite denote_expr_Plus. rewrite interp_imp_bind.
@@ -848,13 +839,13 @@ Section PROOFS.
   Qed.
 
   Lemma interp_imp_expr_Minus
-        ge0 le0 a b
+        ge le0 a b
     :
-      interp_imp ge0 le0 (denote_expr (Minus a b)) =
-      '(le1, (ge1, l)) <- interp_imp ge0 le0 (denote_expr a) ;;
-      '(le2, (ge2, r)) <- interp_imp ge1 le1 (denote_expr b) ;;
+      interp_imp ge le0 (denote_expr (Minus a b)) =
+      '(le1, l) <- interp_imp ge le0 (denote_expr a) ;;
+      '(le2, r) <- interp_imp ge le1 (denote_expr b) ;;
       v <- (vsub l r)? ;;
-      Ret (le2, (ge2, v))
+      Ret (le2, v)
   .
   Proof.
     rewrite denote_expr_Minus. rewrite interp_imp_bind.
@@ -863,13 +854,13 @@ Section PROOFS.
   Qed.
 
   Lemma interp_imp_expr_Mult
-        ge0 le0 a b
+        ge le0 a b
     :
-      interp_imp ge0 le0 (denote_expr (Mult a b)) =
-      '(le1, (ge1, l)) <- interp_imp ge0 le0 (denote_expr a) ;;
-      '(le2, (ge2, r)) <- interp_imp ge1 le1 (denote_expr b) ;;
+      interp_imp ge le0 (denote_expr (Mult a b)) =
+      '(le1, l) <- interp_imp ge le0 (denote_expr a) ;;
+      '(le2, r) <- interp_imp ge le1 (denote_expr b) ;;
       v <- (vmul l r)? ;;
-      Ret (le2, (ge2, v))
+      Ret (le2, v)
   .
   Proof.
     rewrite denote_expr_Mult. rewrite interp_imp_bind.
@@ -878,11 +869,11 @@ Section PROOFS.
   Qed.
 
   Lemma interp_imp_Assign
-        ge0 le0 x e
+        ge le0 x e
     :
-      interp_imp ge0 le0 (denote_stmt (Assign x e)) =
-      '(le1, (ge1, v)) <- interp_imp ge0 le0 (denote_expr e) ;;
-      tau;; tau;; Ret (alist_add _ x v le1, (ge1, Vundef)).
+      interp_imp ge le0 (denote_stmt (Assign x e)) =
+      '(le1, v) <- interp_imp ge le0 (denote_expr e) ;;
+      tau;; tau;; Ret (alist_add _ x v le1, Vundef).
   Proof.
     rewrite denote_stmt_Assign.
     rewrite interp_imp_bind. grind.
@@ -890,94 +881,68 @@ Section PROOFS.
   Qed.
 
   Lemma interp_imp_Seq
-        ge0 le0 a b
+        ge le0 a b
     :
-      interp_imp ge0 le0 (denote_stmt (Seq a b)) =
-      '(le1, (ge1, _)) <- interp_imp ge0 le0 (denote_stmt a) ;;
-      interp_imp ge1 le1 (denote_stmt b).
+      interp_imp ge le0 (denote_stmt (Seq a b)) =
+      '(le1, _) <- interp_imp ge le0 (denote_stmt a) ;;
+      interp_imp ge le1 (denote_stmt b).
   Proof.
     rewrite denote_stmt_Seq.
     apply interp_imp_bind.
   Qed.
 
   Lemma interp_imp_If
-        ge0 le0 i t e
+        ge le0 i t e
     :
-      interp_imp ge0 le0 (denote_stmt (If i t e)) =
-      '(le1, (ge1, v)) <- interp_imp ge0 le0 (denote_expr i) ;;
+      interp_imp ge le0 (denote_stmt (If i t e)) =
+      '(le1, v) <- interp_imp ge le0 (denote_expr i) ;;
       `b: bool <- (is_true v)? ;;
        if b
-       then interp_imp ge1 le1 (denote_stmt t)
-       else interp_imp ge1 le1 (denote_stmt e).
+       then interp_imp ge le1 (denote_stmt t)
+       else interp_imp ge le1 (denote_stmt e).
   Proof.
     rewrite denote_stmt_If. rewrite interp_imp_bind.
     grind. destruct (is_true v); grind; des_ifs.
     unfold interp_imp, interp_GlobEnv, interp_ImpState.
     unfold triggerUB, pure_state. grind.
+    rewrite interp_trigger. grind.
   Qed.
 
-  Lemma _interp_imp_While0
-        ge0 le0 t b
-    :
-      interp_imp ge0 le0 (denote_stmt (While t b)) =
-      interp_imp ge0 le0 (
-        ITree.iter (fun _ => v <- denote_expr t ;; `c: bool <- (is_true v)? ;;
-        if c then (denote_stmt b ;; Ret (inl tt)) else (Ret (inr Vundef)))
-        ()).
-  Proof. reflexivity. Qed.
-
-  (* Lemma interp_imp_iter *)
-  (*       ge0 le0 step *)
-  (*   : *)
-  (*     interp_imp ge0 le0 (ITree.iter step ()) = *)
-  (*     Ret (le0, (ge0, Vundef)). *)
-  (* Proof. *)
-  (*   unfold interp_imp, interp_GlobEnv, interp_ImpState. *)
-  (*   unfold ITree.iter. *)
-  
-  (* Lemma _interp_imp_While *)
-  (*       ge0 le0 t b *)
-  (*   : *)
-  (*     interp_imp ge0 le0 (denote_stmt (While t b)) = *)
-  (*     interp_imp ge0 le0 ( *)
-  (*     while (v <- denote_expr t ;; `c: bool <- (is_true v)? ;; *)
-  (*     if c then (denote_stmt b ;; Ret (inl tt)) else (Ret (inr Vundef)))). *)
-
   Lemma interp_imp_Skip
-        ge0 le0
+        ge le0
     :
-      interp_imp ge0 le0 (denote_stmt (Skip)) =
-      Ret (le0, (ge0, Vundef)).
+      interp_imp ge le0 (denote_stmt (Skip)) =
+      Ret (le0, Vundef).
   Proof.
     rewrite denote_stmt_Skip. apply interp_imp_Ret.
   Qed.
 
   Lemma interp_imp_Return1
-        ge0 le0 e
+        ge le0 e
     :
-      interp_imp ge0 le0 (denote_stmt (Return1 e)) =
-      '(le1, (ge1, v)) <- interp_imp ge0 le0 (denote_expr e) ;;
-      Ret (le1, (ge1, v)).
+      interp_imp ge le0 (denote_stmt (Return1 e)) =
+      '(le1, v) <- interp_imp ge le0 (denote_expr e) ;;
+      Ret (le1, v).
   Proof.
     rewrite denote_stmt_Return1. rewrite interp_imp_bind.
     grind. apply interp_imp_Ret.
   Qed.
 
   Lemma interp_imp_Return2
-        ge0 le0
+        ge le0
     :
-      interp_imp ge0 le0 (denote_stmt (Return2)) =
-      Ret (le0, (ge0, Vundef)).
+      interp_imp ge le0 (denote_stmt (Return2)) =
+      Ret (le0, Vundef).
   Proof.
     rewrite denote_stmt_Return2. apply interp_imp_Ret.
   Qed.
 
   Lemma interp_imp_AddrOf
-        ge0 le0 x X
+        ge le0 x X
     :
-      interp_imp ge0 le0 (denote_stmt (AddrOf x X)) =
-      r <- (ge0.(SkEnv.id2blk) X)? ;; tau;;
-      tau;; tau;; Ret (alist_add _ x (Vptr r 0) le0, (ge0, Vundef)).
+      interp_imp ge le0 (denote_stmt (AddrOf x X)) =
+      r <- (ge.(SkEnv.id2blk) X)? ;; tau;;
+      tau;; tau;; Ret (alist_add _ x (Vptr r 0) le0, Vundef).
   Proof.
     rewrite denote_stmt_AddrOf. rewrite interp_imp_bind.
     rewrite interp_imp_GetPtr. grind.
@@ -985,45 +950,60 @@ Section PROOFS.
   Qed.
 
   Lemma interp_imp_Load
-        ge0 le0 x pe
+        ge le0 x pe
     :
-      interp_imp ge0 le0 (denote_stmt (Load x pe)) =
-      '(le1, (ge1, p)) <- interp_imp ge0 le0 (denote_expr pe);;
+      interp_imp ge le0 (denote_stmt (Load x pe)) =
+      '(le1, p) <- interp_imp ge le0 (denote_expr pe);;
       v <- trigger (Call "load" (p↑));;
       tau;; tau;; v <- unwrapN (v↓);;
-      tau;; tau;; Ret (alist_add _ x v le1, (ge1, Vundef)).
+      tau;; tau;; Ret (alist_add _ x v le1, Vundef).
   Proof.
     rewrite denote_stmt_Load. rewrite interp_imp_bind.
     grind. apply interp_imp_Call_ret.
   Qed.
 
   Lemma interp_imp_Store
-        ge0 le0 pe ve
+        ge le0 pe ve
     :
-      interp_imp ge0 le0 (denote_stmt (Store pe ve)) =
-      '(le1, (ge1, p)) <- interp_imp ge0 le0 (denote_expr pe);;
-      '(le2, (ge2, v)) <- interp_imp ge1 le1 (denote_expr ve);;
-      trigger (Call "store" ([p ; v]↑));; tau;; tau;; Ret (le2, (ge2, Vundef)).
+      interp_imp ge le0 (denote_stmt (Store pe ve)) =
+      '(le1, p) <- interp_imp ge le0 (denote_expr pe);;
+      '(le2, v) <- interp_imp ge le1 (denote_expr ve);;
+      trigger (Call "store" ([p ; v]↑));; tau;; tau;; Ret (le2, Vundef).
   Proof.
     rewrite denote_stmt_Store. rewrite interp_imp_bind.
     grind. rewrite interp_imp_bind. grind.
     apply interp_imp_Call_only.
   Qed.
 
+  Lemma interp_imp_Cmp
+        ge le0 x ae be
+    :
+      interp_imp ge le0 (denote_stmt (Cmp x ae be)) =
+      '(le1, a) <- interp_imp ge le0 (denote_expr ae);;
+      '(le2, b) <- interp_imp ge le1 (denote_expr be);;
+      v <- trigger (Call "cmp" ([a ; b]↑));;
+      tau;; tau;; v <- unwrapN (v↓);;
+      tau;; tau;; Ret (alist_add _ x v le2, Vundef).
+  Proof.
+    rewrite denote_stmt_Cmp. rewrite interp_imp_bind.
+    grind. rewrite interp_imp_bind. grind.
+    apply interp_imp_Call_ret.
+  Qed.
+
   Fixpoint interp_imp_denote_exprs ge le h es acc :=
     match es with
     | [] =>
-      '(le1, (ge1, v)) <- interp_imp ge le (denote_expr h);;
-      Ret (le1, (ge1, v::acc))
+      '(le1, v) <- interp_imp ge le (denote_expr h);;
+      Ret (le1, v::acc)
     | e :: s =>
-      '(le1, (ge1, v)) <- interp_imp ge le (denote_expr h);;
-      interp_imp_denote_exprs ge1 le1 e s (v::acc)
+      '(le1, v) <- interp_imp ge le (denote_expr h);;
+      interp_imp_denote_exprs ge le1 e s (v::acc)
     end.
 
   Lemma interp_imp_exprs
-        ge0 le0 x f args acc
+        ge le0 x f args acc
     :
-      interp_imp ge0 le0 (
+      interp_imp ge le0 (
                    eval_args <- (denote_exprs args acc);;
                    v <- trigger (Call f (eval_args↑));; v <- unwrapN (v↓);;
                    trigger (SetVar x v);; Ret Vundef)
@@ -1032,72 +1012,72 @@ Section PROOFS.
       | [] =>
         v <- trigger (Call f ((acc : list val)↑));;
         tau;; tau;; v <- unwrapN (v↓);;
-        tau;; tau;; Ret (alist_add _ x v le0, (ge0, Vundef))
+        tau;; tau;; Ret (alist_add _ x v le0, Vundef)
       | h::t =>
-        '(le1, (ge1, vs)) <- interp_imp_denote_exprs ge0 le0 h t acc;;
+        '(le1, vs) <- interp_imp_denote_exprs ge le0 h t acc;;
         v <- trigger (Call f (vs↑));;
         tau;; tau;; v <- unwrapN (v↓);;
-        tau;; tau;; Ret (alist_add _ x v le1, (ge1, Vundef))
+        tau;; tau;; Ret (alist_add _ x v le1, Vundef)
       end.
   Proof.
     destruct args.
     - ss. unfold interp_imp, interp_GlobEnv, interp_ImpState. grind.
-      rewrite <- interp_imp_Call_ret.
+      rewrite <- (interp_imp_Call_ret ge).
       unfold interp_imp, interp_GlobEnv, interp_ImpState. grind.
     - move args before Σ. revert_until args. induction args; i.
       + ss. unfold interp_imp, interp_GlobEnv, interp_ImpState. grind.
-        rewrite <- interp_imp_Call_ret.
+        rewrite <- (interp_imp_Call_ret ge).
         unfold interp_imp, interp_GlobEnv, interp_ImpState. grind.
       + ss. grind. rewrite interp_imp_bind. grind.
-        destruct p. ss.
+        destruct x0. ss.
   Qed.
 
   Lemma interp_imp_exprs_only
-        ge0 le0 f args acc
+        ge le0 f args acc
     :
-      interp_imp ge0 le0 (
+      interp_imp ge le0 (
                    eval_args <- (denote_exprs args acc);;
                    trigger (Call f (eval_args↑));; Ret Vundef)
       =
       match args with
       | [] =>
         trigger (Call f ((acc : list val)↑));;
-        tau;; tau;; Ret (le0, (ge0, Vundef))
+        tau;; tau;; Ret (le0, Vundef)
       | h::t =>
-        '(le1, (ge1, vs)) <- interp_imp_denote_exprs ge0 le0 h t acc;;
+        '(le1, vs) <- interp_imp_denote_exprs ge le0 h t acc;;
         trigger (Call f (vs↑));;
-        tau;; tau;; Ret (le1, (ge1, Vundef))
+        tau;; tau;; Ret (le1, Vundef)
       end.
   Proof.
     destruct args.
     - ss. unfold interp_imp, interp_GlobEnv, interp_ImpState. grind.
-      rewrite <- interp_imp_Call_only.
+      rewrite <- (interp_imp_Call_only ge).
       unfold interp_imp, interp_GlobEnv, interp_ImpState. grind.
     - move args before Σ. revert_until args. induction args; i.
       + ss. unfold interp_imp, interp_GlobEnv, interp_ImpState. grind.
-        rewrite <- interp_imp_Call_only.
+        rewrite <- (interp_imp_Call_only ge).
         unfold interp_imp, interp_GlobEnv, interp_ImpState. grind.
       + ss. grind. rewrite interp_imp_bind. grind.
-        destruct p. ss.
+        destruct x. ss.
   Qed.
 
   Lemma interp_imp_CallFun1
-        ge0 le0 x f args
+        ge le0 x f args
     :
-      interp_imp ge0 le0 (denote_stmt (CallFun1 x f args)) =
-      if (String.string_dec f "load" || String.string_dec f "store")
+      interp_imp ge le0 (denote_stmt (CallFun1 x f args)) =
+      if (String.string_dec f "load" || String.string_dec f "store" || String.string_dec f "cmp")
       then triggerUB
       else
         match args with
         | [] =>
           v <- trigger (Call f ([]: list val)↑);;
           tau;; tau;; v <- unwrapN (v↓);;
-          tau;; tau;; Ret (alist_add _ x v le0, (ge0, Vundef))
+          tau;; tau;; Ret (alist_add _ x v le0, Vundef)
         | h::t =>
-          '(le1, (ge1, vs)) <- interp_imp_denote_exprs ge0 le0 h t [];;
+          '(le1, vs) <- interp_imp_denote_exprs ge le0 h t [];;
           v <- trigger (Call f (vs↑));;
           tau;; tau;; v <- unwrapN (v↓);;
-          tau;; tau;; Ret (alist_add _ x v le1, (ge1, Vundef))
+          tau;; tau;; Ret (alist_add _ x v le1, Vundef)
         end.
   Proof.
     rewrite denote_stmt_CallFun1. des_ifs; try (apply interp_imp_exprs).
@@ -1105,20 +1085,20 @@ Section PROOFS.
   Qed.
 
   Lemma interp_imp_CallFun2
-        ge0 le0 f args
+        ge le0 f args
     :
-      interp_imp ge0 le0 (denote_stmt (CallFun2 f args)) =
-      if (String.string_dec f "load" || String.string_dec f "store")
+      interp_imp ge le0 (denote_stmt (CallFun2 f args)) =
+      if (String.string_dec f "load" || String.string_dec f "store" || String.string_dec f "cmp")
       then triggerUB
       else
         match args with
         | [] =>
           trigger (Call f ([]: list val)↑);;
-          tau;; tau;; Ret (le0, (ge0, Vundef))
+          tau;; tau;; Ret (le0, Vundef)
         | h::t =>
-          '(le1, (ge1, vs)) <- interp_imp_denote_exprs ge0 le0 h t [];;
+          '(le1, vs) <- interp_imp_denote_exprs ge le0 h t [];;
           trigger (Call f (vs↑));;
-          tau;; tau;; Ret (le1, (ge1, Vundef))
+          tau;; tau;; Ret (le1, Vundef)
         end.
   Proof.
     rewrite denote_stmt_CallFun2. des_ifs; try (apply interp_imp_exprs_only).
@@ -1126,15 +1106,15 @@ Section PROOFS.
   Qed.
 
   Lemma interp_imp_CallPtr1
-        ge0 le0 x e args
+        ge le0 x e args
     :
-      interp_imp ge0 le0 (denote_stmt (CallPtr1 x e args)) =
-      '(le1, (ge1, p)) <- interp_imp ge0 le0 (denote_expr e);;
+      interp_imp ge le0 (denote_stmt (CallPtr1 x e args)) =
+      '(le1, p) <- interp_imp ge le0 (denote_expr e);;
       match p with
-      | Vptr n _ =>
-        match (SkEnv.blk2id ge1 n) with
+      | Vptr n 0 =>
+        match (SkEnv.blk2id ge n) with
         | Some f =>
-          if (String.string_dec f "load" || String.string_dec f "store")
+          if (String.string_dec f "load" || String.string_dec f "store" || String.string_dec f "cmp")
           then tau;; triggerUB
           else
             match args with
@@ -1142,13 +1122,13 @@ Section PROOFS.
               tau;;
               v <- trigger (Call f ([]: list val)↑);;
               tau;; tau;; v <- unwrapN (v↓);;
-              tau;; tau;; Ret (alist_add _ x v le1, (ge1, Vundef))
+              tau;; tau;; Ret (alist_add _ x v le1, Vundef)
             | h::t =>
               tau;;
-              '(le2, (ge2, vs)) <- interp_imp_denote_exprs ge1 le1 h t [];;
+              '(le2, vs) <- interp_imp_denote_exprs ge le1 h t [];;
               v <- trigger (Call f (vs↑));;
               tau;; tau;; v <- unwrapN (v↓);;
-              tau;; tau;; Ret (alist_add _ x v le2, (ge2, Vundef))
+              tau;; tau;; Ret (alist_add _ x v le2, Vundef)
             end
         | None => triggerUB
         end
@@ -1157,36 +1137,41 @@ Section PROOFS.
   Proof.
     rewrite denote_stmt_CallPtr1. rewrite interp_imp_bind.
     grind. unfold interp_imp, interp_GlobEnv, interp_ImpState. grind.
-    des_ifs; grind.
-    1, 2, 5, 6:( unfold triggerUB, pure_state; grind ).
-    - rewrite <- interp_imp_exprs with (args := []).
+    des_ifs; grind; rewrite interp_trigger.
+    1, 2, 5, 6, 7, 8:( unfold triggerUB, pure_state; grind; unfold triggerUB; grind ).
+    1, 2:( unfold unwrapU, triggerUB; des_ifs; grind; rewrite interp_trigger; grind ).
+    - rewrite <- (interp_imp_exprs ge) with (args := []).
       unfold interp_imp, interp_GlobEnv, interp_ImpState. grind.
-    - rewrite <- interp_imp_exprs with (args := (e0::l0)).
+      unfold pure_state. rewrite interp_trigger. grind.
+      unfold unwrapU, triggerUB; grind.
+      rewrite interp_trigger; grind.
+    - rewrite <- (interp_imp_exprs ge) with (args := (e0::l0)).
       unfold interp_imp, interp_GlobEnv, interp_ImpState. grind.
+      unfold pure_state, unwrapU, triggerUB; grind.
   Qed.
 
   Lemma interp_imp_CallPtr2
-        ge0 le0 e args
+        ge le0 e args
     :
-      interp_imp ge0 le0 (denote_stmt (CallPtr2 e args)) =
-      '(le1, (ge1, p)) <- interp_imp ge0 le0 (denote_expr e);;
+      interp_imp ge le0 (denote_stmt (CallPtr2 e args)) =
+      '(le1, p) <- interp_imp ge le0 (denote_expr e);;
       match p with
-      | Vptr n _ =>
-        match (SkEnv.blk2id ge1 n) with
+      | Vptr n 0 =>
+        match (SkEnv.blk2id ge n) with
         | Some f =>
-          if (String.string_dec f "load" || String.string_dec f "store")
+          if (String.string_dec f "load" || String.string_dec f "store" || String.string_dec f "cmp")
           then tau;; triggerUB
           else
             match args with
             | [] =>
               tau;;
               trigger (Call f ([]: list val)↑);;
-              tau;; tau;; Ret (le1, (ge1, Vundef))
+              tau;; tau;; Ret (le1, Vundef)
             | h::t =>
               tau;;
-              '(le2, (ge2, vs)) <- interp_imp_denote_exprs ge1 le1 h t [];;
+              '(le2, vs) <- interp_imp_denote_exprs ge le1 h t [];;
               trigger (Call f (vs↑));;
-              tau;; tau;; Ret (le2, (ge2, Vundef))
+              tau;; tau;; Ret (le2, Vundef)
             end
         | None => triggerUB
         end
@@ -1195,18 +1180,23 @@ Section PROOFS.
   Proof.
     rewrite denote_stmt_CallPtr2. rewrite interp_imp_bind.
     grind. unfold interp_imp, interp_GlobEnv, interp_ImpState. grind.
-    des_ifs; grind.
-    1, 2, 5, 6:( unfold triggerUB, pure_state; grind ).
-    - rewrite <- interp_imp_exprs_only with (args := []).
+    des_ifs; grind; rewrite interp_trigger.
+    1, 2, 5, 6, 7, 8:( unfold triggerUB, pure_state; grind; unfold triggerUB; grind ).
+    1, 2:( unfold unwrapU, triggerUB; des_ifs; grind; rewrite interp_trigger; grind ).
+    - rewrite <- (interp_imp_exprs_only ge) with (args := []).
       unfold interp_imp, interp_GlobEnv, interp_ImpState. grind.
-    - rewrite <- interp_imp_exprs_only with (args := (e0::l0)).
+      unfold pure_state. rewrite interp_trigger. grind.
+      unfold unwrapU, triggerUB; grind.
+      rewrite interp_trigger; grind.
+    - rewrite <- (interp_imp_exprs_only ge) with (args := (e0::l0)).
       unfold interp_imp, interp_GlobEnv, interp_ImpState. grind.
+      unfold pure_state, unwrapU, triggerUB; grind.
   Qed.
 
   Lemma interp_imp_exprs_sys
-        ge0 le0 x f args acc
+        ge le0 x f args acc
     :
-      interp_imp ge0 le0 (
+      interp_imp ge le0 (
                    eval_args <- (denote_exprs args acc);;
                    v <- trigger (Syscall f eval_args top1);;
                    trigger (SetVar x v);; Ret Vundef)
@@ -1215,88 +1205,88 @@ Section PROOFS.
       | [] =>
         v <- trigger (Syscall f ((acc : list val)) top1);;
         tau;; tau;; tau;; tau;;
-        Ret (alist_add _ x v le0, (ge0, Vundef))
+        Ret (alist_add _ x v le0, Vundef)
       | h::t =>
-        '(le1, (ge1, vs)) <- interp_imp_denote_exprs ge0 le0 h t acc;;
+        '(le1, vs) <- interp_imp_denote_exprs ge le0 h t acc;;
         v <- trigger (Syscall f vs top1);;
         tau;; tau;; tau;; tau;;
-        Ret (alist_add _ x v le1, (ge1, Vundef))
+        Ret (alist_add _ x v le1, Vundef)
       end.
   Proof.
     destruct args.
     - ss. unfold interp_imp, interp_GlobEnv, interp_ImpState. grind.
-      rewrite <- interp_imp_Syscall_ret.
+      rewrite <- (interp_imp_Syscall_ret ge).
       unfold interp_imp, interp_GlobEnv, interp_ImpState. grind.
     - move args before Σ. revert_until args. induction args; i.
       + ss. unfold interp_imp, interp_GlobEnv, interp_ImpState. grind.
-        rewrite <- interp_imp_Syscall_ret.
+        rewrite <- (interp_imp_Syscall_ret ge).
         unfold interp_imp, interp_GlobEnv, interp_ImpState. grind.
       + ss. grind. rewrite interp_imp_bind. grind.
-        destruct p. ss.
+        destruct x0. ss.
   Qed.
 
   Lemma interp_imp_exprs_sys_only
-        ge0 le0 f args acc
+        ge le0 f args acc
     :
-      interp_imp ge0 le0 (
+      interp_imp ge le0 (
                    eval_args <- (denote_exprs args acc);;
                    trigger (Syscall f eval_args top1);; Ret Vundef)
       =
       match args with
       | [] =>
         trigger (Syscall f (acc : list val) top1);;
-        tau;; tau;; Ret (le0, (ge0, Vundef))
+        tau;; tau;; Ret (le0, Vundef)
       | h::t =>
-        '(le1, (ge1, vs)) <- interp_imp_denote_exprs ge0 le0 h t acc;;
+        '(le1, vs) <- interp_imp_denote_exprs ge le0 h t acc;;
         trigger (Syscall f vs top1);;
-        tau;; tau;; Ret (le1, (ge1, Vundef))
+        tau;; tau;; Ret (le1, Vundef)
       end.
   Proof.
     destruct args.
     - ss. unfold interp_imp, interp_GlobEnv, interp_ImpState. grind.
-      rewrite <- interp_imp_Syscall_only.
+      rewrite <- (interp_imp_Syscall_only ge).
       unfold interp_imp, interp_GlobEnv, interp_ImpState. grind.
     - move args before Σ. revert_until args. induction args; i.
       + ss. unfold interp_imp, interp_GlobEnv, interp_ImpState. grind.
-        rewrite <- interp_imp_Syscall_only.
+        rewrite <- (interp_imp_Syscall_only ge).
         unfold interp_imp, interp_GlobEnv, interp_ImpState. grind.
       + ss. grind. rewrite interp_imp_bind. grind.
-        destruct p. ss.
+        destruct x. ss.
   Qed.
 
   Lemma interp_imp_CallSys1
-        ge0 le0 x f args
+        ge le0 x f args
     :
-      interp_imp ge0 le0 (denote_stmt (CallSys1 x f args)) =
+      interp_imp ge le0 (denote_stmt (CallSys1 x f args)) =
       match args with
       | [] =>
         v <- trigger (Syscall f ([]: list val) top1);;
         tau;; tau;; tau;; tau;;
-        Ret (alist_add _ x v le0, (ge0, Vundef))
+        Ret (alist_add _ x v le0, Vundef)
       | h::t =>
-        '(le1, (ge1, vs)) <- interp_imp_denote_exprs ge0 le0 h t [];;
+        '(le1, vs) <- interp_imp_denote_exprs ge le0 h t [];;
         v <- trigger (Syscall f vs top1);;
         tau;; tau;; tau;; tau;;
-        Ret (alist_add _ x v le1, (ge1, Vundef))
+        Ret (alist_add _ x v le1, Vundef)
       end.
   Proof.
     rewrite denote_stmt_CallSys1. apply interp_imp_exprs_sys.
   Qed.
 
   Lemma interp_imp_CallSys2
-        ge0 le0 f args
+        ge le0 f args
     :
-      interp_imp ge0 le0 (denote_stmt (CallSys2 f args)) =
+      interp_imp ge le0 (denote_stmt (CallSys2 f args)) =
       match args with
       | [] =>
         trigger (Syscall f ([]: list val) top1);;
         tau;; tau;;
-        Ret (le0, (ge0, Vundef))
+        Ret (le0, Vundef)
       | h::t =>
-        '(le1, (ge1, vs)) <- interp_imp_denote_exprs ge0 le0 h t [];;
+        '(le1, vs) <- interp_imp_denote_exprs ge le0 h t [];;
         trigger (Syscall f vs top1);;
         tau;; tau;;
-        Ret (le1, (ge1, Vundef))
+        Ret (le1, Vundef)
       end.
   Proof.
     rewrite denote_stmt_CallSys2. apply interp_imp_exprs_sys_only.
@@ -1312,7 +1302,7 @@ Section PROOFS.
                         (match init_args fparams args [] with
                          | Some iargs =>
                            ITree.bind (interp_imp ge (iargs++(init_lenv (fvars))) (denote_stmt fbody))
-                                      (fun x_ : lenv * (_ * val) => let '(_, (_, retv)) := x_ in Ret retv)
+                                      (fun x_ : lenv * val => let '(_, retv) := x_ in Ret retv)
                          | None => triggerUB
                          end) ;; Ret (vret↑).
   Proof. reflexivity. Qed.
@@ -1339,7 +1329,6 @@ Ltac imp_red :=
     | Assign _ _ => rewrite interp_imp_Assign
     | Seq _ _ => rewrite interp_imp_Seq; imp_red
     | If _ _ _ => rewrite interp_imp_If
-    | While _ _ => rewrite _interp_imp_While0 (* need upgrade *)
     | Skip => rewrite interp_imp_Skip
     | CallFun1 _ _ _ => rewrite interp_imp_CallFun1
     | CallFun2 _ _ => rewrite interp_imp_CallFun2
@@ -1352,6 +1341,7 @@ Ltac imp_red :=
     | AddrOf _ _ => rewrite interp_imp_AddrOf
     | Load _ _ => rewrite interp_imp_Load
     | Store _ _ => rewrite interp_imp_Store
+    | Cmp _ _ _ => rewrite interp_imp_Cmp
     | _ => fail
     end
 
